Some refactoring that I did a couple of weeks ago and forgot to commit.

Circuit/CircuitBase.dfy
@@ -1,5 +1,6 @@
 module CircuitBase {
 
+    import Utils
     import opened Std.Wrappers
     import Std.Collections.Seq
 
@@ -35,7 +36,7 @@ module CircuitBase {
         //NodeBound: CNode,
         //PortBound: CPort,
         HierLevel: nat,
-        PortNames: map<string, CNode>
+        PortMap: PortMapping
     )
 
     function NodeKind(c: Circuit, n: CNode): Option<CNodeKind>
@@ -59,11 +60,9 @@ module CircuitBase {
       | CHier(c: Circuit)
         // A node representing combinatorial logic.
       | CComb(
-          IPorts: seq<CPort>,
-          OPorts: seq<CPort>,
           PathExists: (CPort, CPort) -> bool,
           Behav: map<CPort, bool> -> Option<map<CPort, bool>>,
-          PortNames: string -> Option<CPort>
+          PortMap: PortMapping
         )
         // A contant 0 or 1
       | CConst(value: bool)
@@ -74,18 +73,36 @@ module CircuitBase {
         // A register.
       | CSeq()
 
-    function IPorts(nk: CNodeKind): set<CPort>
+    function PortMap(nk: CNodeKind): PortMapping
     {
         match nk
-        // The port numbers of a hierarical block and just the node ids of
-        // the input and output nodes.
-        case CHier(subc) =>
-            set n | n in subc.NodeKind && subc.NodeKind[n] == CInput :: n as CPort
-        case CComb(iports, oports, path_exists, behav, names) => Seq.ToSet(iports)
-        case CInput() => {}
-        case CConst(v) => {}
-        case COutput() => {INPUT_PORT as CPort}
-        case CSeq() => {INPUT_PORT as CPort}
+        case CHier(_) => nk.c.PortMap
+        case CComb(_, _, _) => nk.PortMap
+        case CConst(_) => PortMapping([], [], ["o"], [OUTPUT_PORT])
+        case CInput() => PortMapping([], [], ["o"], [OUTPUT_PORT])
+        case COutput() => PortMapping(["i"], [INPUT_PORT], [], [])
+        case CSeq() => PortMapping(["i"], [INPUT_PORT], ["o"], [OUTPUT_PORT])
+    }
+
+    function PortNameToPort(nk: CNodeKind, name: string): CPort
+        requires CNodeKindSomewhatValid(nk)
+        requires
+            var pm := PortMap(nk);
+            name in pm.inames || name in pm.onames
+    {
+        var pm := PortMap(nk);
+        assert PortMappingValid(pm);
+        if name in pm.inames then
+            INameToPort(pm, name)
+        else
+            assert name in pm.onames;
+            ONameToPort(pm, name)
+    }
+
+    function IPorts(nk: CNodeKind): set<CPort>
+    {
+        var pm := PortMap(nk);
+        Seq.ToSet(pm.iports)
     }
 
     predicate IsPort(nk: CNodeKind, p: CPort)
@@ -99,72 +116,72 @@ module CircuitBase {
     {
         reveal Seq.ToSet();
     }
+
     lemma InOPortsIsOPort(nk: CNodeKind, p: CPort)
         requires IsOPort(nk, p)
         ensures p in OPorts(nk)
     {
         reveal Seq.ToSet();
-        match nk
-        case CHier(subc) => {}
-        case CComb(iports, oports, path_exists, behav, name) => {}
-        case CInput() => {}
-        case CConst(v) => {}
-        case COutput() => {}
-        case CSeq() => {}
     }
 
     predicate IsIPort(nk: CNodeKind, p: CPort)
     {
-        match nk
-        // The port numbers of a hierarical block and just the node ids of
-        // the input and output nodes.
-        case CHier(subc) => NodeKind(subc, p as CNode) == Some(CInput)
-        case CComb(iports, oports, path_exists, behav, name) => p in iports
-        case CInput() => false
-        case CConst(v) => false
-        case COutput() => p == INPUT_PORT as CPort
-        case CSeq() => p == INPUT_PORT as CPort
+        var pm := PortMap(nk);
+        p in pm.iports
+
+        //match nk
+        //// The port numbers of a hierarical block and just the node ids of
+        //// the input and output nodes.
+        //case CHier(subc) => NodeKind(subc, p as CNode) == Some(CInput)
+        //case CComb(path_exists, behav, pm) => p in pm.iports
+        //case CInput() => false
+        //case CConst(v) => false
+        //case COutput() => p == INPUT_PORT as CPort
+        //case CSeq() => p == INPUT_PORT as CPort
     }
 
     function OPorts(nk: CNodeKind): set<CPort>
     {
-        match nk
-        case CHier(subc) =>
-            set n | n in subc.NodeKind && subc.NodeKind[n] == COutput :: n as CPort
-        case CComb(iports, oports, path_exists, behav, names) => Seq.ToSet(oports)
-        case CInput() => {OUTPUT_PORT as CPort}
-        case COutput() => {}
-        case CConst(v) => {OUTPUT_PORT as CPort}
-        case CSeq() => {OUTPUT_PORT as CPort}
+        var pm := PortMap(nk);
+        Seq.ToSet(pm.oports)
+
+        //match nk
+        //case CHier(subc) =>
+        //    set n | n in subc.NodeKind && subc.NodeKind[n] == COutput :: n as CPort
+        //case CComb(path_exists, behav, pm) => Seq.ToSet(pm.oports)
+        //case CInput() => {OUTPUT_PORT as CPort}
+        //case COutput() => {}
+        //case CConst(v) => {OUTPUT_PORT as CPort}
+        //case CSeq() => {OUTPUT_PORT as CPort}
     }
 
     predicate IsOPort(nk: CNodeKind, p: CPort)
     {
-        match nk
-        // The port numbers of a hierarical block and just the node ids of
-        // the input and output nodes.
-        case CHier(subc) =>
-            NodeKind(subc, p as CNode) == Some(COutput)
-        case CComb(iports, oports, path_exists, behav, names) => p in oports
-        case CInput() => p == OUTPUT_PORT as CPort
-        case CConst(v) => p == OUTPUT_PORT as CPort
-        case COutput() => false
-        case CSeq() => p == OUTPUT_PORT as CPort
+        var pm := PortMap(nk);
+        p in pm.oports
+        //match nk
+        //// The port numbers of a hierarical block and just the node ids of
+        //// the input and output nodes.
+        //case CHier(subc) =>
+        //    NodeKind(subc, p as CNode) == Some(COutput)
+        //case CComb(path_exists, behav, pm) => p in pm.oports
+        //case CInput() => p == OUTPUT_PORT as CPort
+        //case CConst(v) => p == OUTPUT_PORT as CPort
+        //case COutput() => false
+        //case CSeq() => p == OUTPUT_PORT as CPort
     }
 
     ghost predicate CNodeKindSomewhatValid(nk: CNodeKind)
     {
         (
         match nk
-        case CComb(iports, oports, path_exists, behav, names) =>
+        case CComb(path_exists, behav, pm) =>
           (forall a: CPort, b: CPort ::
-              (a !in oports ==> !nk.PathExists(a, b)) &&
-              (b !in iports ==> !nk.PathExists(a, b)))
+              (a !in pm.oports ==> !nk.PathExists(a, b)) &&
+              (b !in pm.iports ==> !nk.PathExists(a, b)))
         case _ => true
-        ) && (
-            forall p: CPort ::
-                !(IsIPort(nk, p) && IsOPort(nk, p))
-        )
+        ) &&
+        PortMappingValid(PortMap(nk))
     }
 
     lemma CNodeKindNoSelfPaths(nk: CNodeKind)
@@ -175,6 +192,9 @@ module CircuitBase {
         forall p: CPort
             ensures !nk.PathExists(p, p)
         {
+            var pm := PortMap(nk);
+            assert PortMappingValid(nk.PortMap);
+            assert !(p in pm.iports && p in pm.oports);
             assert !(IsIPort(nk, p) && IsOPort(nk, p));
         }
     }
@@ -197,18 +217,34 @@ module CircuitBase {
         decreases  c.HierLevel, 2
     {
         CircuitNodeKindValid(c) &&
-        CircuitPortSourceValid(c)
+        CircuitPortSourceValid(c) &&
+        CircuitPortNamesValid(c)
+    }
+
+    ghost predicate {:opaque} CircuitPortNamesValid(c: Circuit)
+    {
+        (forall s :: s in c.PortMap.iports <==> CNodeIsCInput(c, s as CNode)) &&
+        (forall s :: s in c.PortMap.oports <==> CNodeIsCOutput(c, s as CNode)) &&
+        PortMappingValid(c.PortMap)
+    }
+
+    lemma CircuitUpdatedCircuitNodeKindValid(c: Circuit, new_c: Circuit)
+        requires CircuitValid(c)
+        requires new_c.NodeKind == c.NodeKind
+        requires new_c.HierLevel == c.HierLevel
+        ensures CircuitNodeKindValid(new_c)
+    {
+        reveal CircuitValid();
     }
 
     ghost predicate CircuitNodeKindValid(c: Circuit)
         decreases  c.HierLevel, 1
     {
         forall n: CNode ::
-            var maybe_nk := NodeKind(c, n);
-            if maybe_nk.None? then
+            if n !in c.NodeKind then
                 true
             else
-                CNodeKindValid(c.HierLevel, maybe_nk.Extract())
+                CNodeKindValid(c.HierLevel, c.NodeKind[n])
     }
 
     ghost predicate CircuitPortSourceValid(c: Circuit)
@@ -217,18 +253,19 @@ module CircuitBase {
         // If the port is not a valid output port then PortSource should give None.0
         // If the port is a valid output port then it should lead to a valid input
         // port.
-        forall n: CNode ::
-            forall p: CPort ::
-                var inp := NP(n, p);
-                if NPValidInput(c, inp) then
-                    match PortSource(c, inp)
+        forall n: CNode, p: CPort ::
+            var inp := NP(n, p);
+            if NPValidInput(c, inp) then
+                if inp in c.PortSource then
+                    var onp := c.PortSource[inp];
+                    NPValidOutput(c, onp)
+                else
                     // It's ok if it doesn't connect to anything.
                     // We consider that a valid circuit, but not a complete circuit.
                     // That way we can build a circuit but it is still valid.
-                    case None => true
-                    case Some(onp) => NPValidOutput(c, onp)
-                else
-                    PortSource(c, inp) == None
+                    true
+            else
+                inp !in c.PortSource
     }
 
     ghost predicate NPValid(c: Circuit, np: NP)
@@ -264,6 +301,85 @@ module CircuitBase {
     predicate CNodeIsCOutput(c: Circuit, n: CNode)
     {
         NodeKind(c, n).Some? && NodeKind(c, n).value.COutput?
+    }
+
+    datatype PortMapping =
+        PortMapping(
+            inames: seq<string>,
+            iports: seq<CPort>,
+            onames: seq<string>,
+            oports: seq<CPort>
+        )
+
+    predicate PortMappingValid(m: PortMapping)
+    {
+        |m.inames| == |m.iports| &&
+        (forall i: nat, j: nat :: i < |m.inames| && j < |m.inames| && i != j ==>
+            m.inames[i] != m.inames[j] && m.iports[i] != m.iports[j]) &&
+        |m.onames| == |m.oports| &&
+        (forall i: nat, j: nat :: i < |m.onames| && j < |m.onames| && i != j ==>
+            m.onames[i] != m.onames[j] && m.oports[i] != m.oports[j]) &&
+        (forall i: nat, j: nat :: i < |m.inames| && j < |m.onames| ==>
+            m.inames[i] != m.onames[j] && m.iports[i] != m.oports[j])
+    }
+
+    function INameToPort(m: PortMapping, name: string): CPort
+        requires PortMappingValid(m)
+        requires name in m.inames
+    {
+        var index := Seq.IndexOf(m.inames, name);
+        m.iports[index]
+    }
+
+    lemma INameToPortCovers(m: PortMapping)
+        requires PortMappingValid(m)
+        ensures
+            var inames: set<string> := (set k | k in m.inames);
+            var iports := (set k | k in inames :: INameToPort(m, k));
+            forall k :: k in iports <==> k in m.iports
+    {
+            var iports := seq(|m.inames|, (i: nat) requires i < |m.inames| =>
+                INameToPort(m, m.inames[i]));
+            assert iports == m.iports;
+    }
+
+    function ONameToPort(m: PortMapping, name: string): CPort
+        requires PortMappingValid(m)
+        requires name in m.onames
+    {
+        var index := Seq.IndexOf(m.onames, name);
+        m.oports[index]
+    }
+
+    function PortMappingAddIPort(pm: PortMapping, s: string, p: CPort): (r: PortMapping)
+        requires PortMappingValid(pm)
+        requires s !in pm.inames
+        requires s !in pm.onames
+        requires p !in pm.iports
+        requires p !in pm.oports
+    {
+        PortMapping(
+            inames := pm.inames + [s],
+            iports := pm.iports + [p],
+            onames := pm.onames,
+            oports := pm.oports
+        )
+    }
+
+    function PortMappingAddOPort(pm: PortMapping, s: string, p: CPort): (r: PortMapping)
+        requires PortMappingValid(pm)
+        requires s !in pm.inames
+        requires s !in pm.onames
+        requires p !in pm.iports
+        requires p !in pm.oports
+        ensures PortMappingValid(r)
+    {
+        PortMapping(
+            inames := pm.inames,
+            iports := pm.iports,
+            onames := pm.onames + [s],
+            oports := pm.oports + [p]
+        )
     }
 
 }
