Circuit/CircuitEvaluate.dfy
@@ -7,7 +7,7 @@ module CircuitEvaluate {
     import opened CircuitHierarchy
     import opened CircuitToGraph
     import DG = DigraphBase`Spec
-    import DP = DigraphPaths
+    import DP = DigraphPaths`Spec
 
     function {:vcs_split_on_every_assert} EvaluateINP(
             c: Circuit, m: HPNP -> bool, p: DG.Path<HPNP>): bool
@@ -110,10 +110,150 @@ module CircuitEvaluate {
         match nk
         case CInput() => EvaluateONPCInput(c, isigs, p)
         case CHier(_) => EvaluateONPCHier(c, isigs, p)
-        case CComb(_, _, _, _, _) => EvaluateONPCComb(c, isigs, p)
+        case CComb(_, _, _) => EvaluateONPCComb(c, isigs, p)
         case CSeq() => isigs(onp)
         case CConst(v) => v
     }
 
-}
+    ghost predicate StringInputMapValid(c: Circuit, inputmap: map<string, bool>)
+    {
+        forall s :: s in inputmap <==> s in c.PortMap.inames
+    }
 
+    ghost predicate StringOutputMapValid(c: Circuit, outputmap: map<string, bool>)
+    {
+        forall s :: s in outputmap <==> s in c.PortMap.onames
+    }
+
+    ghost predicate CNodeInputMapValid(c: Circuit, inputmap: map<CNode, bool>)
+    {
+        forall n :: n in inputmap <==> CNodeIsCInput(c, n)
+    }
+
+    ghost predicate CNodeOutputMapValid(c: Circuit, outputmap: map<CNode, bool>)
+    {
+        forall n :: n in outputmap <==> CNodeIsCOutput(c, n)
+    }
+
+    function StringMapToPortMap(c: Circuit, inputmap: map<string, bool>): (r: map<CNode, bool>)
+        requires CircuitValid(c)
+        requires StringInputMapValid(c, inputmap)
+        ensures CNodeInputMapValid(c, r)
+    {
+        reveal CircuitValid();
+        reveal CircuitPortNamesValid();
+        INameToPortCovers(c.PortMap);
+        assert forall p :: (p in c.PortMap.iports <==> CNodeIsCInput(c, p as CNode));
+        var iports := (set k | k in c.PortMap.inames :: INameToPort(c.PortMap, k) as CNode);
+        assert forall p :: p in iports <==> p as CPort in c.PortMap.iports;
+        assert forall p :: p in iports ==> CNodeIsCInput(c, p);
+        var r := (map k | k in c.PortMap.inames :: INameToPort(c.PortMap, k) as CNode := inputmap[k]);
+        assert forall k :: k in r.Keys <==> k in iports;
+        assert forall k :: k in r.Keys ==> CNodeIsCInput(c, k);
+        assert forall k :: CNodeIsCInput(c, k) ==> k in r.Keys;
+        r
+    }
+
+    function PortMapToHPNPMap(inputmap: map<CNode, bool>): HPNP -> bool
+    {
+        var outputmap := (hpnp: HPNP) => hpnp.hpn.hp == HP([]) && hpnp.hpn.n in inputmap && hpnp.p == OUTPUT_PORT && inputmap[hpnp.hpn.n];
+        outputmap
+    }
+
+    function InputLabelToHPNP(c: Circuit, input_label: string): (r: HPNP)
+        requires CircuitValid(c)
+        requires input_label in c.PortMap.inames
+        ensures HPNPValidOutput(c, r)
+    {
+        reveal CircuitValid();
+        reveal CircuitPortNamesValid();
+        var n := INameToPort(c.PortMap, input_label) as CNode;
+        assert n as CPort in c.PortMap.iports;
+        assert CNodeIsCInput(c, n);
+        reveal HPNPValidOutput();
+        HPNP(HPNode(HP([]), n), OUTPUT_PORT)
+    }
+
+    function OutputLabelToHPNP(c: Circuit, output_label: string): (r: HPNP)
+        requires CircuitValid(c)
+        requires output_label in c.PortMap.onames
+        ensures HPNPValidInput(c, r)
+    {
+        reveal CircuitValid();
+        reveal CircuitPortNamesValid();
+        var n := ONameToPort(c.PortMap, output_label) as CNode;
+        assert n as CPort in c.PortMap.oports;
+        assert CNodeIsCOutput(c, n);
+        reveal HPNPValidInput();
+        var r := HPNP(HPNode(HP([]), n), INPUT_PORT);
+        //HierarchyPathValid(c, hpnp.hpn.hp) &&
+        //var hp_c := HierarchyPathCircuit(c, hpnp.hpn.hp);
+        //var maybe_nk := NodeKind(hp_c, hpnp.hpn.n);
+        //maybe_nk.Some? &&
+        //IsIPort(maybe_nk.value, hpnp.p)
+        assert r.p in PortMap(COutput).iports;
+        assert IsIPort(COutput, r.p);
+        assert HPNPValidInput(c, r);
+        r
+    }
+
+    lemma EvaluateByLabelHelper(c: Circuit, output_label: string)
+        requires CircuitValid(c)
+        requires output_label in c.PortMap.onames
+        ensures PathValid(c, DG.Path([OutputLabelToHPNP(c, output_label)]))
+    {
+        var hpnp := OutputLabelToHPNP(c, output_label);
+        assert HPNPValidInput(c, hpnp);
+        reveal HPNPValidInput();
+        reveal DG.PathValid();
+        reveal CtoG();
+        var p := DG.Path([hpnp]);
+        var g := CtoGV(c);
+        assert HPNPValid(c, hpnp);
+        ValidHPNPIsNode(c, hpnp);
+        assert hpnp in AllValidHPNP(c);
+        assert DG.IsNode(g, hpnp);
+        assert DG.PathValid(g, p);
+        assert PathValid(c, p);
+    }
+
+    lemma EvaluateByLabelHelper2(c: Circuit)
+        requires CircuitValid(c)
+        ensures forall input_label :: input_label in c.PortMap.onames ==> PathValid(c, DG.Path([OutputLabelToHPNP(c, input_label)]))
+    {
+        forall output_label | output_label in c.PortMap.onames
+            ensures PathValid(c, DG.Path([OutputLabelToHPNP(c, output_label)]))
+        {
+            EvaluateByLabelHelper(c, output_label);
+        }
+    }
+
+    //function EvaluateByPort(c: Circuit, inputmap: map<CNode, bool>): (r: map<CNode, bool>)
+    //    requires CircuitValid(c)
+    //    requires CircuitNoLoops(c)
+    //    requires CircuitComplete(c)
+    //    requires CNodeInputMapValid(c, inputmap)
+    //    ensures CNodeOutputMapValid(c, r)
+    //{
+    //    var m := PortMapToHPNPMap(inputmap);
+    //    reveal DG.PathValid();
+    //    reveal CtoG();
+    //    EvaluateByLabelHelper2(c);
+    //    (map k | k in c.PortMap.oports :: k as CNode := EvaluateINP(c, m, DG.Path([HPNP(HPNode(HP([]), k as CNode), INPUT_PORT)])))
+    //}
+
+    function EvaluateByLabel(c: Circuit, inputmap: map<string, bool>): (r: map<string, bool>)
+        requires CircuitValid(c)
+        requires CircuitNoLoops(c)
+        requires CircuitComplete(c)
+        requires StringInputMapValid(c, inputmap)
+        ensures StringOutputMapValid(c, r)
+    {
+        var m := PortMapToHPNPMap(StringMapToPortMap(c, inputmap));
+        reveal DG.PathValid();
+        reveal CtoG();
+        EvaluateByLabelHelper2(c);
+        (map k | k in c.PortMap.onames :: k := EvaluateINP(c, m, DG.Path([OutputLabelToHPNP(c, k)])))
+    }
+
+}
