Digraph/DigraphStepBack.dfy
@@ -1,14 +1,22 @@
 module DigraphStepBack {
 
-    export Body
-        provides DBS
-        reveals StepBack
-
     import opened Std.Wrappers
+    import Std.Collections.Seq
+    import Std.Relations
 
+    import SetExt
+
+    import DBB=DigraphBase`Body
     import DBS=DigraphBase`Spec
     import opened DigraphBase`Body
     import opened DigraphPaths`Body
+
+    export Body
+        provides DBB // FIXME: Can we avoid providing the body.
+        reveals MultipleStepSetBack
+        reveals StepSetBack
+        reveals StepSetBackInternal
+        reveals StepBack
 
     lemma NoPathLengthXNoPathsLonger<Node>(g: Digraph, length: nat)
         requires !exists p: Path<Node> :: |p.v| == length && PathValid(g, p)
@@ -42,12 +50,12 @@ module DigraphStepBack {
             r
     }
 
-    lemma MultipleStepSetEmptyGivesNoLoop<Node(!new)>(g: Digraph, count: nat)
+    lemma MultipleStepSetEmptyGivesNoLoop<Node(!new)>(g: Digraph, count: nat, NodeOrdering: (Node, Node) -> bool)
         requires DigraphValid(g)
-        requires MultipleStepSetBack(g, AllNodes(g), count) == {}
+        requires MultipleStepSetBack(g, AllNodes(g), count, NodeOrdering) == {}
         ensures !DigraphLoop(g)
     {
-        MultipleStepSetBackGivesMaxPathLength(g, count);
+        MultipleStepSetBackGivesMaxPathLength(g, count, NodeOrdering);
         reveal DigraphLoop();
         reveal PathValid();
         if DigraphLoop(g) {
@@ -56,18 +64,17 @@ module DigraphStepBack {
         }
     }
 
-    lemma {:vcs_split_on_every_assert} MultipleStepSetBackGivesMaxPathLength<Node(!new)>(g: Digraph, count: nat)
+    lemma {:vcs_split_on_every_assert} MultipleStepSetBackGivesMaxPathLength<Node(!new)>(g: Digraph, count: nat, NodeOrdering: (Node, Node) -> bool)
         requires DigraphValid(g)
-        requires MultipleStepSetBack(g, AllNodes(g), count) == {}
+        requires MultipleStepSetBack(g, AllNodes(g), count, NodeOrdering) == {}
         ensures forall p : Path<Node> :: PathValid(g, p) ==> |p.v| <= count
     {
         // We want to show that if the input set is all nodes and the result is an empty set then the maximum path length is <= 'count'.
         reveal PathValid();
         var all_nodes := AllNodes(g);
-
         if count == 0 {
-            assert MultipleStepSetBack(g, AllNodes(g), count) == all_nodes;
-            assert all_nodes == {};
+            assert MultipleStepSetBack(g, all_nodes, count, NodeOrdering) == all_nodes;
+            assert all_nodes == {}; 
         }
 
         if exists p: Path<Node> :: |p.v| == count+1 && PathValid(g, p) {
@@ -80,7 +87,7 @@ module DigraphStepBack {
                     assert false;
                 }
             } else {
-                PathExistsEndInMultipleStepSet(g, p, all_nodes);
+                PathExistsEndInMultipleStepSet(g, p, all_nodes, NodeOrdering);
             }
             assert forall p : Path<Node> :: PathValid(g, p) ==> |p.v| <= count;
         } else {
@@ -90,18 +97,18 @@ module DigraphStepBack {
         }
     }
 
-    ghost function MultipleStepSetBack<Node(!new)>(g: Digraph, in_ns: set<Node>, count: nat): (r: set<Node>)
+    function MultipleStepSetBack<Node(!new)>(g: Digraph, in_ns: set<Node>, count: nat, NodeOrdering: (Node, Node) -> bool): (r: set<Node>)
         requires DigraphValid(g)
         decreases count
     {
         if count == 0 then
             in_ns
         else
-            var s := StepSetBack(g, in_ns);
-            MultipleStepSetBack(g, s, count-1)
+            var s := StepSetBack(g, in_ns, NodeOrdering);
+            MultipleStepSetBack(g, s, count-1, NodeOrdering)
     }
 
-    ghost function StepSetBackInternal<Node(!new)>(g: Digraph, in_ns: set<Node>, out_ns: set<Node>): (r: set<Node>)
+    function StepSetBackInternal<Node(!new)>(g: Digraph, in_ns: set<Node>, out_ns: set<Node>, NodeOrdering: (Node, Node) -> bool): (r: set<Node>)
         requires DigraphValid(g)
         ensures forall m :: (m in r <==> (exists n :: n in in_ns && IsConnected(g, n, m)) || (m in out_ns))
     {
@@ -109,34 +116,35 @@ module DigraphStepBack {
             var r := out_ns;
             r
         else
-            var n :| n in in_ns;
+            var n := SetExt.GetMin(in_ns, NodeOrdering);
             var connected := StepBack(g, n);
             assert forall m :: (m in connected ==> IsConnected(g, n, m));
             var new_in_ns := in_ns - {n};
             var new_out_ns := out_ns + connected;
-            var r := StepSetBackInternal(g, new_in_ns, new_out_ns);
+            var r := StepSetBackInternal(g, new_in_ns, new_out_ns, NodeOrdering);
             r
     }
 
-    ghost function StepSetBack<Node(!new)>(g: Digraph, in_ns: set<Node>): (r: set<Node>)
+    function StepSetBack<Node(!new)>(g: Digraph, in_ns: set<Node>, NodeOrdering: (Node, Node)->bool): (r: set<Node>)
         // Returns a set of all the nodes that there nodes are connected to
         requires DigraphValid(g)
         ensures forall m :: m in r <==> exists n :: (n in in_ns && IsConnected(g, n, m))
     {
-        StepSetBackInternal(g, in_ns, {})
+        StepSetBackInternal(g, in_ns, {}, NodeOrdering)
     }
 
-    lemma {:vcs_split_on_every_assert} PathExistsEndInMultipleStepSet<Node(!new)>(g: Digraph, p: Path<Node>, in_ns: set<Node>)
+    lemma {:vcs_split_on_every_assert} PathExistsEndInMultipleStepSet<Node(!new)>(g: Digraph, p: Path<Node>, in_ns: set<Node>, NodeOrdering: (Node, Node) -> bool)
+        requires Relations.TotalOrdering(NodeOrdering)
         requires DigraphValid(g)
         requires PathValid(g, p)
         requires |p.v| > 0
         requires PathStart(p) in in_ns
         ensures
-            var out_s := MultipleStepSetBack(g, in_ns, |p.v|-1);
+            var out_s := MultipleStepSetBack(g, in_ns, |p.v|-1, NodeOrdering);
             PathEnd(p) in out_s
         decreases |p.v|
     {
-        var out_ns := MultipleStepSetBack(g, in_ns, |p.v|-1);
+        var out_ns := MultipleStepSetBack(g, in_ns, |p.v|-1, NodeOrdering);
         if |p.v| == 1 {
             assert out_ns == in_ns;
             assert PathEnd(p) == PathStart(p);
@@ -144,11 +152,11 @@ module DigraphStepBack {
         } else {
             var head := PathStart(p);
             var tail := Path(p.v[1..]);
-            var intermed_ns := StepSetBack(g, in_ns);
+            var intermed_ns := StepSetBack(g, in_ns, NodeOrdering);
             reveal PathValid();
             assert IsConnected(g, head, PathStart(tail));
             assert PathStart(tail) in intermed_ns;
-            PathExistsEndInMultipleStepSet(g, tail, intermed_ns);
+            PathExistsEndInMultipleStepSet(g, tail, intermed_ns, NodeOrdering);
         }
     }
     
